<?xml version="1.0"?>


<!DOCTYPE rdf:RDF [
    <!ENTITY dct "http://purl.org/dc/terms/" >
    <!ENTITY owl "http://www.w3.org/2002/07/owl#" >
    <!ENTITY dc "http://purl.org/dc/elements/1.1/" >
    <!ENTITY xsd "http://www.w3.org/2001/XMLSchema#" >
    <!ENTITY rdfs "http://www.w3.org/2000/01/rdf-schema#" >
    <!ENTITY rdf "http://www.w3.org/1999/02/22-rdf-syntax-ns#" >
]>


<rdf:RDF xmlns="http://purl.oclc.org/NET/iot#"
     xml:base="http://purl.oclc.org/NET/iot"
     xmlns:dct="http://purl.org/dc/terms/"
     xmlns:rdf="http://www.w3.org/1999/02/22-rdf-syntax-ns#"
     xmlns:owl="http://www.w3.org/2002/07/owl#"
     xmlns:xsd="http://www.w3.org/2001/XMLSchema#"
     xmlns:rdfs="http://www.w3.org/2000/01/rdf-schema#"
     xmlns:dc="http://purl.org/dc/elements/1.1/">
    <owl:Ontology rdf:about="http://purl.oclc.org/NET/iot">
        <dc:identifier>http://purl.oclc.org/NET/iot</dc:identifier>
        <dct:created>2015-06-30</dct:created>
        <dc:title>Semantic Internet of Things Ontology</dc:title>
        <rdfs:comment>Semantic Internet of Things ontology that extends the Semantic Sensor Ontology for Internet of Things devices</rdfs:comment>
        <owl:imports rdf:resource="http://purl.oclc.org/NET/ssnx/ssn"/>
        <owl:imports rdf:resource="http://www.w3.org/2006/time"/>
    </owl:Ontology>
    


    <!-- 
    ///////////////////////////////////////////////////////////////////////////////////////
    //
    // Data properties
    //
    ///////////////////////////////////////////////////////////////////////////////////////
     -->

    


    <!-- http://purl.oclc.org/NET/iot#hasQuantityValue -->

    <owl:DatatypeProperty rdf:about="http://purl.oclc.org/NET/iot#hasQuantityValue">
        <rdfs:domain rdf:resource="http://purl.oclc.org/NET/iot#QuantityObservationValue"/>
        <rdfs:subPropertyOf rdf:resource="http://www.loa-cnr.it/ontologies/DUL.owl#hasDataValue"/>
    </owl:DatatypeProperty>
    


    <!-- 
    ///////////////////////////////////////////////////////////////////////////////////////
    //
    // Classes
    //
    ///////////////////////////////////////////////////////////////////////////////////////
     -->

    


    <!-- http://purl.oclc.org/NET/iot#ExternalTemperatureValue -->

    <owl:Class rdf:about="http://purl.oclc.org/NET/iot#ExternalTemperatureValue">
        <rdfs:label>External Temperature Value</rdfs:label>
        <rdfs:subClassOf rdf:resource="http://purl.oclc.org/NET/iot#QuantityObservationValue"/>
        <rdfs:comment>The external temperature measured from the environment, not within an enclosed area.</rdfs:comment>
    </owl:Class>
    


    <!-- http://purl.oclc.org/NET/iot#InternalTemperatureValue -->

    <owl:Class rdf:about="http://purl.oclc.org/NET/iot#InternalTemperatureValue">
        <rdfs:label>Internal Temperature Value</rdfs:label>
        <rdfs:subClassOf rdf:resource="http://purl.oclc.org/NET/iot#QuantityObservationValue"/>
        <rdfs:comment>An internal temperature value within an enclosed area.</rdfs:comment>
    </owl:Class>
    


    <!-- http://purl.oclc.org/NET/iot#QuantityObservationValue -->

    <owl:Class rdf:about="http://purl.oclc.org/NET/iot#QuantityObservationValue">
        <rdfs:label>Quantity observation value</rdfs:label>
        <rdfs:subClassOf rdf:resource="http://purl.oclc.org/NET/ssnx/ssn#ObservationValue"/>
        <rdfs:subClassOf>
            <owl:Restriction>
                <owl:onProperty rdf:resource="http://purl.oclc.org/NET/iot#hasQuantityValue"/>
                <owl:cardinality rdf:datatype="&xsd;nonNegativeInteger">1</owl:cardinality>
            </owl:Restriction>
        </rdfs:subClassOf>
        <rdfs:comment>Enables the extension of ssn:ObservationValue to provide assertions on units of measurement, etc.</rdfs:comment>
    </owl:Class>
    


    <!-- http://purl.oclc.org/NET/iot#WeatherObservation -->

    <owl:Class rdf:about="http://purl.oclc.org/NET/iot#WeatherObservation">
        <rdfs:label>Weather Observation</rdfs:label>
        <rdfs:subClassOf rdf:resource="http://purl.oclc.org/NET/ssnx/ssn#Observation"/>
        <rdfs:subClassOf>
            <owl:Restriction>
                <owl:onProperty rdf:resource="http://purl.oclc.org/NET/ssnx/ssn#observedBy"/>
                <owl:allValuesFrom rdf:resource="http://purl.oclc.org/NET/iot#WeatherSensor"/>
            </owl:Restriction>
        </rdfs:subClassOf>
        <rdfs:subClassOf>
            <owl:Restriction>
                <owl:onProperty rdf:resource="http://purl.oclc.org/NET/ssnx/ssn#observationResult"/>
                <owl:allValuesFrom rdf:resource="http://purl.oclc.org/NET/iot#WeatherSensorOutput"/>
            </owl:Restriction>
        </rdfs:subClassOf>
        <rdfs:subClassOf>
            <owl:Restriction>
                <owl:onProperty rdf:resource="http://purl.oclc.org/NET/ssnx/ssn#observationSamplingTime"/>
                <owl:allValuesFrom rdf:resource="http://www.w3.org/2006/time#Instant"/>
            </owl:Restriction>
        </rdfs:subClassOf>
        <rdfs:comment>A class describing weather observations. Properties ssn:observationResult, ssn:observationSamplingTime and ssn:observedBy are restricted accordingly.</rdfs:comment>
    </owl:Class>
    


    <!-- http://purl.oclc.org/NET/iot#WeatherSensor -->

    <owl:Class rdf:about="http://purl.oclc.org/NET/iot#WeatherSensor">
        <rdfs:label>Weather Sensor</rdfs:label>
        <rdfs:subClassOf rdf:resource="http://purl.oclc.org/NET/ssnx/ssn#SensingDevice"/>
        <rdfs:comment>WeatherSensor is a subclass of sensing devices which measures various effects of the weather like temperature, humidity, rain or wind.</rdfs:comment>
    </owl:Class>
    


    <!-- http://purl.oclc.org/NET/iot#WeatherSensorOutput -->

    <owl:Class rdf:about="http://purl.oclc.org/NET/iot#WeatherSensorOutput">
        <rdfs:label>Weather sensor output</rdfs:label>
        <rdfs:subClassOf rdf:resource="http://purl.oclc.org/NET/ssnx/ssn#SensorOutput"/>
        <rdfs:subClassOf>
            <owl:Restriction>
                <owl:onProperty rdf:resource="http://purl.oclc.org/NET/ssnx/ssn#isProducedBy"/>
                <owl:allValuesFrom rdf:resource="http://purl.oclc.org/NET/iot#WeatherSensor"/>
            </owl:Restriction>
        </rdfs:subClassOf>
        <rdfs:subClassOf>
            <owl:Restriction>
                <owl:onProperty rdf:resource="http://purl.oclc.org/NET/ssnx/ssn#hasValue"/>
                <owl:allValuesFrom>
                    <owl:Class>
                        <owl:unionOf rdf:parseType="Collection">
                            <rdf:Description rdf:about="http://purl.oclc.org/NET/iot#ExternalTemperatureValue"/>
                            <rdf:Description rdf:about="http://purl.oclc.org/NET/iot#InternalTemperatureValue"/>
                        </owl:unionOf>
                    </owl:Class>
                </owl:allValuesFrom>
            </owl:Restriction>
        </rdfs:subClassOf>
        <rdfs:comment>A class describing sensor output for measurements from a weather sensor. Properties ssn:hasValue and ssn:isProducedBy are restricted accordingly.</rdfs:comment>
    </owl:Class>
</rdf:RDF>



<!-- Generated by the OWL API (version 3.5.1) http://owlapi.sourceforge.net -->

